Build.v
@@ -20,6 +20,15 @@ Section Build.
 Variable maxReg : nat.          (* max number of registers *)
 Definition PhysReg : predArgType := 'I_maxReg.
 
+Variables blockType1 blockType2 opType1 opType2 accType : Set.
+
+Variable binfo : BlockInfo blockType1 blockType2 opType1 opType2.
+Variable oinfo : OpInfo maxReg accType opType1 opType2.
+
+Definition BuildState (b : nat) := IntMap (SortedRanges b.*2.+1).
+
+Definition newBuildState {n} : BuildState n := emptyIntMap.
+
 (* block   range   first    last      range   ranges   ranges   block
    beg     beg     use pos  use pos   end     beg      end      end
    |       |       |              |       |   |             |       |
@@ -49,57 +58,46 @@ Definition PhysReg : predArgType := 'I_maxReg.
    include the range; otherwise, the new range is prepended normally into the
    sorted list of ranges. *)
 
-Record BuildState (b : nat) := {
-  bsVars : IntMap (SortedRanges b.*2.+1)
+Record RangeCursor b pos e := {
+  cursorMid : nat;
+  cursorHmid : pos.*2.+1 <= cursorMid.*2.+1;
+  cursorHbeg : b.*2.+1 <= pos.*2.+1;
+  cursorPending : BoundedRange b.*2.+1 cursorMid.*2.+1;
+  cursorHpos : pos.*2.+1 <= head_or_end cursorPending.1.1;
+  cursorRanges : SortedRanges cursorMid.*2.+1;
+  cursorHend :
+    last cursorMid.*2.+1 [seq rend i.1 | i <- cursorRanges.1] <= e.*2.+1
 }.
 
-Definition newBuildState {n} : BuildState n :=
-  {| bsVars := emptyIntMap |}.
-
-Variables blockType1 blockType2 opType1 opType2 accType : Set.
-
-Variable binfo : BlockInfo blockType1 blockType2 opType1 opType2.
-Variable oinfo : OpInfo maxReg accType opType1 opType2.
-
-Definition RangeCursor b pos mid e :=
-  { p : BoundedRange b.*2.+1 mid.*2.+1 * SortedRanges mid.*2.+1
-  | let r := (fst p).1.1 in
-    [&& last mid.*2.+1 [seq rend i.1 | i <- (snd p).1] <= e.*2.+1
-    ,   b.*2.+1 <= pos.*2.+1
-    &   pos.*2.+1 <= head_or_end r ] }.
-
 Definition emptyRangeCursor (b pos e : nat) (H : b < pos <= e) :
-  RangeCursor b pos pos e.
+  RangeCursor b pos e.
 Proof.
   have Hsz : b.*2.+1 < pos.*2.+1 by undoubled.
-  exists (emptyBoundedRange Hsz (odd_double_plus _),
-          emptySortedRanges) => /=.
-  by undoubled.
+  apply: {| cursorMid := pos |} => //=.
+  - by ordered.
+  - exact: (emptyBoundedRange Hsz (odd_double_plus _)).
+  - by [].
+  - exact: emptySortedRanges.
+  - by undoubled.
 Defined.
 
-Definition transportRangeCursor {b prev base mid e}
+Definition transportRangeCursor {b prev base e}
   (Hlt : b.*2.+1 <= base.*2.+1 <= prev.*2.+1)
-  (c : RangeCursor b prev mid e) :
-  RangeCursor b base mid e.
+  (c : RangeCursor b prev e) : RangeCursor b base e.
 Proof.
-  case: c => [[r /= rs] H1] in Hlt *.
-  apply: (exist _ (r, rs) _) => /=.
-  by case: (ups r.1.1) => /= [|u us] in H1 *; ordered.
+  case: c => [mid ? ? r /= Hpos rs ?] in Hlt *.
+  apply: {| cursorMid := mid |} => //=;
+  by case: (ups r.1.1) => /= [|u us] in Hpos *; ordered.
 Defined.
-
-Definition FloatingCursor b pos e :=
-  { p : { n : nat | pos <= n } & RangeCursor b pos p.1 e }.
 
 Definition PendingRanges b pos e :=
-  { _ : IntMap (FloatingCursor b pos e) | b.*2.+1 <= pos.*2.+1 <= e.*2.+1 }.
+  { _ : IntMap (RangeCursor b pos e) | b.*2.+1 <= pos.*2.+1 <= e.*2.+1 }.
 
 Definition emptyPendingRanges (b pos e : nat) (H : b < pos <= e)
   (liveOuts : IntSet) : PendingRanges b pos e.
 Proof.
   have empty  := emptyRangeCursor H.
-  have empty' : FloatingCursor b pos e :=
-    (existT _ (exist _ pos (leqnn pos)) empty).
-  have f xs vid := IntMap_insert vid empty' xs.
+  have f xs vid := IntMap_insert vid empty xs.
   exists (IntSet_foldl f emptyIntMap liveOuts).
   by undoubled.
 Defined.
@@ -110,17 +108,16 @@ Definition mergeIntoSortedRanges `(H : b <= pos)
 Proof.
   apply: (IntMap_mergeWithKey _ _ _ pmap.1 rmap).
   - (* The combining function, when entries are present in both maps. *)
-    move=> _ [[mid Hmid] /= [[br ps] /= Hlt]] rs.
+    move=> _ [mid Hmid H1 br /= H2 ps H3] rs.
     have H0: b.*2.+1 <= b.*2.+1 <= rbeg br.1.1.
       move: (Range_beg_bounded br.1.2).
-      move: br => [r Hr] /= in Hlt *.
+      move: br => [r Hr] /= in H2 *.
       by case: (ups r.1); ordered.
-    move/andP: Hlt => [H1 /andP [H2 H3]].
     pose ps' := prependRange ps H0.
     move: ps' => [ps' spec].
     clear H0.
     apply: (Some (@SortedRanges_cat _ ps' _ rs _)) => /=.
-    move: br => [r Hlt] in H3 ps' spec *.
+    move: br => [r Hlt] in H2 ps' spec *.
     have H4: rend r.1 <= mid.*2.+1.
       have Hlt' := Hlt.
       by ordered.
@@ -128,16 +125,16 @@ Proof.
       have Hlt' := Hlt.
       move: (Range_bounded r.2) => ?.
       by ordered.
-    have p := last_leq H1 H4.
+    have p := last_leq H3 H4.
     rewrite spec /= in p.
     exact: (last_leq p H5).
 
   - (* When no rmap entry are present. *)
     apply: IntMap_map _.
-    case=> [[? _] /= [[br rs] _]].
+    case=> [? _ /= ? br Hpos rs ?].
     have H0: b.*2.+1 <= b.*2.+1 <= rbeg br.1.1.
       move: (Range_beg_bounded br.1.2).
-      move: br => [r ?] /=.
+      move: br => [r ?] /= in Hpos *.
       by case: (ups r.1); ordered.
     exact: (prependRange rs H0).1.
 
@@ -157,10 +154,10 @@ Definition varKindLtn (x y : VarKind) : bool :=
   end.
 
 Definition handleVars_combine {b pos e} (H : b <= pos) (vid : nat)
-  (range : FloatingCursor b pos.+1 e) (vars : bool * seq VarKind) :
-  option (FloatingCursor b pos e).
+  (range : RangeCursor b pos.+1 e) (vars : bool * seq VarKind) :
+  option (RangeCursor b pos e).
 Proof.
-  move: range => [[mid Hmid] [[br srs] /= /andP [H1 /andP [H2 H3]]]].
+  move: range => [mid Hmid H1 br /= H2 srs H3].
   move: vars => [req kinds].
 
   set upos := {| uloc   := pos.*2.+1
@@ -169,13 +166,13 @@ Proof.
 
   have E: (upos < head_or_end br.1.1).
     rewrite /=.
-    by case: (ups br.1.1) => /= [|u us] in H3 *; undoubled.
+    by case: (ups br.1.1) => /= [|u us] in H2 *; undoubled.
 
   have Hupos: match ups br.1.1 with
       | [::]   => upos < rend br.1.1
       | u :: _ => upos <= u
       end.
-    by case: (ups br.1.1) => /= [|u us] in H3 E *; undoubled.
+    by case: (ups br.1.1) => /= [|u us] in H2 E *; undoubled.
 
   case K: ((Output \in kinds) && (Input \notin kinds)).
   - (* If this is an output variable that is not also used as an input
@@ -183,7 +180,7 @@ Proof.
        use position into that range.  We also shift up the beginning of the
        range, since it may begin here.  By doing this iteratively for each
        variable, we determine when the range truly starts. *)
-    move: br srs => [r Hr] [rs Hsort Hlt] /= in H1 H3 E Hupos *.
+    move: br srs => [r Hr] [rs Hsort Hlt] /= in H2 H3 E Hupos *.
     pose r1 := Range_shiftup (b:=upos) r.2 Hodd Hupos.
 
     have Hloc: rbeg r1.1 <= upos < head_or_end r1.1.
@@ -195,17 +192,13 @@ Proof.
     pose r2 := Range_cons Hodd r1.2 Hloc.
 
     rewrite /= in H1 Hloc r2.
-    clear H3 E r1; simpl in *.
-    apply: Some (existT _ (exist _ mid (ltnW Hmid))
-                   (exist _
-                      (exist _ r2 _,
-                       exist2 _ _ rs _ _) _)) => /=.
-    + apply/andP; split.
-        by undoubled.
-      clear -Hr.
-      by ordered.
-    + move/andP=> [? ?].
-      by ordered.
+    apply: Some {| cursorMid     := mid
+                 ; cursorPending := exist _ r2 _
+                 ; cursorRanges  := exist2 _ _ rs _ _
+                 |} => //=.
+    + by ordered.
+    + by undoubled.
+    + by undoubled.
 
   - (* Otherwise, we must create a new [BoundedRange], and merge the previous
        one into the [SortedRanges]. *)
@@ -213,16 +206,15 @@ Proof.
     + have U: rbeg br.1.1 <= upos < head_or_end br.1.1
         by ordered.
       pose r1 := Range_cons Hodd br.1.2 U.
-      apply: Some _.
-      apply: existT _ (exist _ mid _) _ => //=.
-        by ordered.
-      move=> _.
-      apply: exist _ (exist _ r1 _, srs) _ => /=.
+      apply: Some {| cursorMid     := mid
+                   ; cursorPending := exist _ r1 _
+                   ; cursorRanges  := srs
+                   |} => //=.
+      * by ordered.
+      * by undoubled.
       * clear -br.
         move: br => [? Hr].
         exact: Hr.
-      * move=> Hr.
-        by undoubled.
 
     + pose r1 := newRange Hodd.
 
@@ -237,22 +229,21 @@ Proof.
         apply: ltn_odd => //.
         by apply/andP; split.
 
-      apply: Some (existT _ (exist _ pos.+1 _)
-                     (exist _
-                        (exist _ r1 _, _) _)) => //= _.
+      apply: Some {| cursorMid     := pos.+1
+                   ; cursorPending := exist _ r1 _
+                   |} => //=.
+      * by ordered.
+      * by undoubled.
       * by undoubled.
       * exact: (prependRange srs Hspan).1.
-      * move=> _.
-        case: (prependRange srs Hspan) => [p /= spec].
-        apply/andP; split=> /=;
-          last by undoubled.
+      * case: (prependRange srs Hspan) => [p /= spec].
         have Hmid': (pos.+1).*2.+1 <= mid.*2.+1.
           by undoubled.
-        move: br => [r Hlt] in H3 spec E Hupos Hloc Hspan *.
+        move: br => [r Hlt] in H2 spec E Hupos Hloc Hspan *.
         have H4: rend r.1 <= mid.*2.+1.
           pose Hlt' := Hlt.
           by ordered.
-        have Hleq := last_leq H1 H4.
+        have Hleq := last_leq H3 H4.
         rewrite spec /= in Hleq.
         apply: (last_leq Hleq _).
         move: (Range_bounded r.2).
@@ -261,16 +252,14 @@ Defined.
 
 Definition handleVars_onlyRanges {b pos e}
   (Hlt : b.*2.+1 <= pos.*2.+1 <= (pos.+1).*2.+1) :
-  IntMap (FloatingCursor b pos.+1 e) -> IntMap (FloatingCursor b pos e).
+  IntMap (RangeCursor b pos.+1 e) -> IntMap (RangeCursor b pos e).
 Proof.
   apply: IntMap_map _.
-  move=> [[mid Hmid] cursor].
-  move: (transportRangeCursor Hlt cursor) => cursor'.
-  exact: existT _ (exist _ mid (ltnW Hmid)) _.
+  exact: (transportRangeCursor Hlt).
 Defined.
 
 Definition handleVars_onlyVars {b pos e} (H1 : b <= pos < e) :
-  IntMap (bool * seq VarKind) -> IntMap (FloatingCursor b pos e).
+  IntMap (bool * seq VarKind) -> IntMap (RangeCursor b pos e).
 Proof.
   apply: IntMap_map _.
   move=> [req kinds].
@@ -287,11 +276,10 @@ Proof.
      ; ups  := [:: {| uloc   := pos.*2.+1
                     ; regReq := req |} ]
      |}.
-  apply: existT _ (exist _ e _) _ => /=.
-    by ordered.
-  move=> Hmid.
-
-  apply: exist _ (exist _ (exist _ rd _) _, _) _ => /=.
+  apply: {| cursorMid     := e
+          ; cursorPending := exist _ (exist _ rd _) _
+          |} => //=;
+  try undoubled.
   - constructor=> /=.
     + by case: (Input \in kinds); undoubled.
     + by case: (Output \in kinds); undoubled.
@@ -304,8 +292,7 @@ Proof.
     by undoubled.
   - exists [::] => //.
     by constructor.
-  - move=> r H /=.
-    by undoubled.
+  - by undoubled.
 Defined.
 
 Definition extractVarInfo (xs : seq (VarInfo maxReg)) : bool * seq VarKind :=
@@ -394,8 +381,7 @@ Proof.
   have Hsze : pos < endpos <= endpos by ordered.
 
   have pending := reduceBlock (emptyPendingRanges Hsze outs).
-  exact: {| bsVars := mergeIntoSortedRanges (ltnW Hsz) pending
-                                            (bsVars (IHbs endpos)) |}.
+  exact: mergeIntoSortedRanges (ltnW Hsz) pending (IHbs endpos).
 Defined.
 
 Definition compileIntervals `(bs : BuildState pos) :
@@ -403,7 +389,7 @@ Definition compileIntervals `(bs : BuildState pos) :
      respectively. *)
   FixedIntervalsType maxReg * IntMap IntervalSig.
 Proof.
-  apply: IntMap_foldlWithKey _ (vconst None, emptyIntMap) (bsVars bs).
+  apply: IntMap_foldlWithKey _ (vconst None, emptyIntMap) bs.
   move=> [regs vars] vid rs.
   case E: rs.1 => [|? ?]; first by exact: (regs, vars).
   case V: (vid < maxReg).
@@ -418,7 +404,6 @@ Definition buildIntervals (blocks : seq blockType1)
   (liveSets : IntMap BlockLiveSets) : SSError + ScanStateSig maxReg InUse :=
   let handleVar (ss  : ScanStateSig maxReg Pending) i :=
         packScanState (ScanState_newUnhandled ss.2 i.2 I) in
-
   let s0 := ScanState_nil maxReg in
   if blocks isn't b :: bs
   then inr $ packScanState (ScanState_finalize s0)
